[WIP] Fiddling with proof / security condition likely to discard this

experimental/ni_coq/vfiles/EvAugSemanticsDwn.v
@@ -21,87 +21,87 @@ Inductive step_node_ev (id: node_id): call -> state -> down_l ->
     | SWriteChanEv s nlbl han msg s':
         (s.(nodes) .[?id]).(lbl) = nlbl ->
         step_node id (WriteChannel han msg) s s' ->
-        step_node_ev id (WriteChannel han msg) s (ell DWN nil)
+        step_node_ev id (WriteChannel han msg) s (nlbl DWNnil)
             s' (nlbl ---> msg)
         (* The notations used for events on this last line and others
         is in Events.v *)
     | SWriteChanDwnEv s nlbl han msg s' ell':
         (s.(nodes) .[?id]).(lbl) = nlbl ->
-        step_node id (WriteChannel han msg ell') s s' ->
-        step_node_ev id (WriteChannel han msg ell') s (msg DWN nlbl |--> ell')
+        step_node id (WriteChannelDown han msg ell') s s' ->
+        step_node_ev id (WriteChannelDown han msg ell') s (msg DWN nlbl |--> ell')
             s' (nlbl ---> msg)
     | SReadChanEv s nlbl han chan msg s':
         (s.(nodes) .[?id]).(lbl) = nlbl ->
         step_node id (ReadChannel han) s s' ->
         msg_is_head chan msg ->
-        step_node_ev id (ReadChannel han) s (ell DWN nil)
+        step_node_ev id (ReadChannel han) s (nlbl DWNnil)
             s' (nlbl <--- msg)
     | SCreateChanEv s nlbl clbl s':
         (* It seems clear that no event is needed since nodes only observe
         * contents of channels indirectly via reads *)
         (s.(nodes) .[?id]).(lbl) = nlbl ->
         step_node id (CreateChannel clbl) s s' ->
-        step_node_ev id (CreateChannel clbl) s (ell DWN nil)
+        step_node_ev id (CreateChannel clbl) s (nlbl DWNnil)
             s' (nlbl --- )
     | SCreateNodeEv s nlbl new_lbl h s':
         (s.(nodes) .[?id]).(lbl) = nlbl ->
         step_node id (CreateNode new_lbl h) s s' ->
-        step_node_ev id (CreateNode new_lbl h) s (ell DWN nil)
+        step_node_ev id (CreateNode new_lbl h) s (nlbl DWNnil)
             s' ( -- nlbl -- )
     | SWaitOnChannelsEv s hs nlbl s':
         (s.(nodes) .[?id]).(lbl) = nlbl ->
         step_node id (WaitOnChannels hs) s s' ->
-        step_node_ev id (WaitOnChannels hs) s (ell DWN nil)
+        step_node_ev id (WaitOnChannels hs) s (nlbl DWNnil)
             s' (nlbl ---)
     | SChannelCloseEv s han nlbl s':
         (s.(nodes) .[?id]).(lbl) = nlbl ->
         step_node id (ChannelClose han) s s' ->
-        step_node_ev id (ChannelClose han) s (ell DWN nil)
+        step_node_ev id (ChannelClose han) s (nlbl DWNnil)
             s' (nlbl ---)
     | SNodeLabelReadEv s nlbl s':
         (s.(nodes) .[?id]).(lbl) = nlbl ->
         step_node id NodeLabelRead s s' ->
-        step_node_ev id NodeLabelRead s (ell DWN nil)
+        step_node_ev id NodeLabelRead s (nlbl DWNnil)
             s' (nlbl <--L nlbl)
     | SChannelLabelReadEv s han nlbl clbl s':
         (s.(nodes) .[?id]).(lbl) = nlbl ->
         (s.(chans) .[?han]).(lbl) = clbl ->
         step_node id (ChannelLabelRead han) s s' ->
-        step_node_ev id (ChannelLabelRead han) s (ell DWN nil)
+        step_node_ev id (ChannelLabelRead han) s (nlbl DWNnil)
             s' (nlbl <--L clbl)
     | SInternalEv s nlbl s':
         (s.(nodes) .[?id]).(lbl) = nlbl ->
         step_node id Internal s s' ->
-        step_node_ev id Internal s (ell DWN nil)
+        step_node_ev id Internal s (nlbl DWNnil)
             s' (nlbl ---).
 
-Inductive step_system_ev: state -> state -> event_l -> Prop :=
-    | SytsemEvSkip s ell: step_system_ev s s (ell ---) 
-    | SystemEvStepNode id n c c' s s' e:
+Inductive step_system_ev: state -> down_l -> state -> event_l -> Prop :=
+    | SytsemEvSkip s ell: step_system_ev s (ell DWNnil) s (ell ---) 
+    | SystemEvStepNode id n c c' s d s' e:
         (s.(nodes).[?id]).(obj) = Some n ->
         n.(ncall) = c ->
-        step_node_ev id c s s' e ->
+        step_node_ev id c s d s' e ->
         let s'' := (s_set_call s' id c') in
             (* Here c' is an arbitrary command. The next ABI call
             that the node makes after the one executed here is an arbitrary one
             of that node's choosing *)
-        step_system_ev s s'' e.
+        step_system_ev s d s'' e.
 
-Definition trace := list (state * event_l).
+Definition trace := list (state * down_l * event_l).
 
 (* This is used for state/event pairs in EvAug. 
 * The type is slightly awkward now post refactor *)
 Definition head_st (t: trace) :=
-    match t with 
+    match t with
         | nil => None
-        | (s', _)::_ => Some s'
+        | (s', _, _)::_ => Some s'
     end.
 
 Inductive step_system_ev_t: trace -> trace -> Prop :=
-    | StepTrace t s s' e:
+    | StepTrace t s d s' e:
         head_st t = Some s -> 
-        step_system_ev s s' e ->
-        step_system_ev_t t ((s', e) :: t).
+        step_system_ev s d s' e ->
+        step_system_ev_t t ((s', d, e) :: t).
 
 Inductive step_system_ev_multi: trace -> trace -> Prop :=
     | multi_system_ev_refl t t':
