experimental/ni_coq/vfiles/EscapeHatchCondition_proof.v
@@ -1,0 +1,86 @@
+Require Import Coq.Lists.List.
+Import ListNotations.
+From OakIFC Require Import
+    Lattice
+    Parameters
+    GenericMap
+    RuntimeModel
+    ModelSemUtils
+    EvAugSemanticsDwn
+    State
+    Events
+    LowEquivalences
+    TraceLowEq
+    TraceTheoremsDwn
+    NIUtilTheorems
+    Unwind
+    EscapeHatchCondition_def 
+    Tactics.
+From RecordUpdate Require Import RecordSet.
+Import RecordSetNotations.
+Local Open Scope map_scope.
+Local Open Scope ev_notation.
+
+
+Hint Resolve multi_system_ev_refl multi_system_ev_tran : multi.
+
+(* hints for eauto in event part of the unobservable step proof *)
+Hint Extern 4 (low_proj _ _  = _ ) => erewrite nflows_labeled_proj : unobs_ev.
+Hint Extern 4 (_  = low_proj _ _ ) => erewrite nflows_labeled_proj : unobs_ev.
+Hint Extern 4 (event_low_eq _ _ _) => unfold event_low_eq : unobs_ev.
+Hint Extern 4 (low_eq _ _ _) => unfold low_eq : unobs_ev.
+
+Definition empty_event (ell: level) := Labeled event None ell.
+
+Theorem escape_hatch_1step: forall ell s1 s2 s1' d1 d2 e1,
+    (state_low_eq ell s1 s2) ->
+    (down_low_eq ell d1 d2) ->
+    (step_system_ev s1 d1 s1' e1) ->
+    (exists s2' e2,
+        (step_system_ev s2 d2 s2' e2) /\
+        (state_low_eq ell s1' s2') /\
+        (event_low_eq ell e1 e2)).
+Proof.
+Admitted.
+
+Theorem escape_hatch_unwind_t: forall ell t1 t2 dt1 dt2 t1',
+(eh_trace_low_eq ell t1 t2) ->
+(down_list_low_eq ell dt1 dt2) ->
+(step_system_ev_t t1 t1') ->
+(dt1 = (extract_downgrade_trace t1')) ->
+(exists t2',
+    (step_system_ev_t t2 t2') /\
+    (dt2 = (extract_downgrade_trace t2')) /\
+    (eh_trace_low_eq ell t1' t2')).
+Proof.
+    intros. 
+    inversion H; crush.
+    -  (* starts from empty trace *)
+        exfalso. eapply no_steps_from_empty; eauto.
+    - (* non-empty trace *)
+        inversion H1; inversion H2; crush.
+        inversion H0. crush.
+        pose proof escape_hatch_1step.
+        pose proof (escape_hatch_1step _ s s2 s' d _ _
+            ltac:(eauto) ltac:(eauto) ltac:(eauto)).
+        pose proof (escape_hatch_1step _ s s2 s' _ _ _
+            ltac:(eauto) ltac:(eauto) ltac:(eauto)) as [s2' [e2' [H2step [Hsleq Heleq]]]].
+        eexists ((s2', d3, e2') :: (s2, d2, e2) :: t3); repeat split; crush.
+        econstructor; crush; eauto.
+        unfold extract_downgrade_trace in *.
+        admit. (* extract trace is = *)
+        econstructor; crush; eauto.
+Admitted.
+
+
+Theorem escape_hatch: (conjecture_escape_hatch step_system_ev_multi).
+Proof.
+  unfold conjecture_escape_hatch. crush.
+  let H := match goal with H : step_system_ev_multi _ _ |- _ => H end in
+  induction H; crush.
+  all:pose proof (escape_hatch_unwind_t
+                    _ _ _ _
+                    ltac:(eassumption) ltac:(eassumption)).
+  all:crush.
+  all:eexists; split; crush; [ | eassumption ]; eauto with multi.
+Qed.
